\documentclass{jhwhw}
\author{Ian Malerich}
\title{Homework: Lambda Calculus \& Racket}
\usepackage{amssymb}

\begin{document}

\problem{}

Given

\begin{tabular}{r@{:}l}
	0&\ \lambda f.\lambda x.x \\
	succ&\ \lambda n.\lambda f. \lambda x.$(f ((n f) x))$ \\
	n&\ if n is a natural number then its semantics is the result of n applications of succ on 0. \\
	true&\ \lambda x.\lambda y.x \\
	false&\ \lambda x.\lambda y.y \\
	second&\ \lambda x.\lambda y. \lambda z.y \\
	g&\ \lambda n.$((n second) false)$ \\
\end{tabular}
\bigbreak
\raggedright
What is the result of

\begin{enumerate}
	\item (g n) when n is 0.
	\item (g n) when n results from some application succ on 0.
	\item What mathematical/logical operation is computed by g.
\end{enumerate}

\solution

\problem{}

Consider the following \lambda$-expression$:

\begin{gather*}
Y : \lambda$t.($\lambda$x.(t (x x)) $\lambda$x.(t (x x)))$
\end{gather*}
Prove/disprove that (Y t) after application of several \beta$-reductions results in (t (Y t))$.

\solution

Setup \\
	\setlength\parindent{24pt}
	We are given (Y t), apply the definition of Y to this given lambda expression. \\
	(\lambda$t.($\lambda$x.(t (x x)) $\lambda$x.(t (x x)))$ $ t)$ \\
	Denote Q: \lambda $x.(t (x x))$ \\
	Note that (Q Q) after a single \beta$-reduction results in (t (Q Q))$ \\
	Thus we are starting with (t (Q Q)).

	\bigbreak
	\setlength\parindent{0pt}
	Claim \\
		\setlength\parindent{24pt}
		let n $\in$ $\lamtbb{N}$ \\
		After n $\beta$-reductions of (t (Q Q)) denoted R \\
		then R $\neq$ (t (Y t)) \\
	 
	\bigbreak
	\setlength\parindent{0pt}
	Proof by Induction on n \\
	\setlength\parindent{24pt}
		Base Case (n = 0) \\
		\setlength\parindent{48pt}
		This is true as Q $\neq$ Y $\wedge$ Q $\neq$ t \\
		Thus (Q Q) $\neq$ (Y t) \\
		Therefore (t (Q Q)) $\neq $ (t (Y t)) \\
		\setlength\parindent{24pt}
		Induction Hypothesis \\
		\setlength\parindent{48pt}
		Assume ($t_0$ ($t_1$ ($\ldots$ ($t_n$ (Q Q))))) $\neq$ (t (Y t)) \\
		\setlength\parindent{24pt}
		Induction Step \\
		\setlength\parindent{48pt}
		We have ($t_0$ ($t_1$ ($\ldots$ ($t_n$ (Q Q))))) $\neq$ (t (Y t)) \\
		Apply a single $\beta$-reduction to the left hand side producing \\
		($t_0$ ($t_1$ ($\ldots$ ($t_n$ ($t_{n+1}$ (Q Q)))))) \\
		(Q Q) $\neq$ (Y t) as proven in the base case. \\
		($t_0$ ($t_1$ ($\ldots$ ($t_n$ ($t_{n+1}$ (X)))))) $\neq$ (t (X)) for any X \\
		as ($t_n$ (\ldots)) is not a lambda expression that can be $\beta$-reduced. \\
		Therefore ($t_0$ ($t_1$ ($\ldots$ ($t_n$ ($t_{n+1}$ (Q Q)))))) $\neq$ (t (Y t)) \square\\

\end{document}
